adding defintions for the lh256 uh256

dfy_model/MultiplyExpr256.dfy
@@ -15,31 +15,27 @@ module MultiplyExpr256 {
     const B5 : int := B * B * B * B * B;
     const B6 : int := B * B * B * B * B * B;
 
-    // lemma shift_test(x: uint32)
-    // {
-    //     var shifted :bv16 := ((x as bv32) >> 16) as bv16;
-    //     assert 0 <= shifted as int < 65536;
-    // }
-
-    function method {:opaque} lh(x: uint256) : uint128
+    function method {:opaque} lh256(x: uint256) : uint128
     {
-        assume false;
-        (x as bv256 & 0xffffffffffffffffffffffffffffffff) as uint128
+        (x % B2) as uint128
     }
 
- 	function method {:opaque} uh(x: uint256) : uint128
+ 	function method {:opaque} uh256(x: uint256) : uint128
     {
-        assume false;
-        (x as bv256 >> 128) as uint128
+        (x / B2) as uint128
     }
 
- 	lemma split_lemma(x: uint256)
- 	 	ensures uh(x) * B2 + lh(x) == x;
- 	 	ensures lh(x) == x % B2;
+ 	lemma split_lemma_256(x: uint256)
+ 	 	ensures uh256(x) * B2 + lh256(x) == x;
+    {
+        reveal lh256();
+        reveal uh256();
+    }
 
     function method mul_limb(a: uint64, b: uint64) : (p: uint128)
         ensures p == a as int * b as int;
     {
+        assume false;
         a as uint128 * b as uint128
     }
 
@@ -56,9 +52,9 @@ module MultiplyExpr256 {
         var a0 :uint256 := mul_limb(a[0], b[0]);
         var a1 :uint256 := a0 + mul_limb(a[1], b[0]) * B;
         var a2 :uint256 := a1 + mul_limb(a[0], b[1]) * B;
-        c_01 := lh(a2);
+        c_01 := lh256(a2);
 
-        var a3 :uint256 := uh(a2) + mul_limb(a[2], b[0]);
+        var a3 :uint256 := uh256(a2) + mul_limb(a[2], b[0]);
         var a4 :uint256 := a3 + mul_limb(a[1], b[1]);
         var a5 :uint256 := a4 + mul_limb(a[0], b[2]);
 
@@ -66,18 +62,18 @@ module MultiplyExpr256 {
         var a7 :uint256 := a6 + mul_limb(a[2], b[1]) * B;
         var a8 :uint256 := a7 + mul_limb(a[1], b[2]) * B;
         var a9 :uint256 := a8 + mul_limb(a[0], b[3]) * B;
-        c_23 := lh(a9);
+        c_23 := lh256(a9);
 
-        var a10 :uint256 := uh(a9) + mul_limb(a[3], b[1]);
+        var a10 :uint256 := uh256(a9) + mul_limb(a[3], b[1]);
         var a11 :uint256 := a10 + mul_limb(a[2], b[2]);
         var a12 :uint256 := a11 + mul_limb(a[1], b[3]);
 
         var a13 :uint256 := a12 + mul_limb(a[3], b[2]) * B;
         var a14 :uint256 := a13 + mul_limb(a[2], b[3]) * B;
-        d_01 := lh(a14);
+        d_01 := lh256(a14);
 
-        var a15 :uint256 := uh(a14) + mul_limb(a[3], b[3]);
-        d_23 := lh(a15);
+        var a15 :uint256 := uh256(a14) + mul_limb(a[3], b[3]);
+        d_23 := lh256(a15);
 
         assume d_23 == a15;
         test_full_mul_lemma(a, b, a2, a9, a14, a15, c_01, c_23, d_01, d_23);
@@ -91,14 +87,14 @@ module MultiplyExpr256 {
         requires a2 == a[0] * b[0] + 
             a[1] * b[0] * B + a[0] * b[1] * B;
         requires a9== a[2] * b[0] + a[1] * b[1] + a[0] * b[2] +
-            a[3] * b[0] * B + a[2] * b[1] * B + a[1] * b[2] * B + a[0] * b[3] * B + uh(a2);
+            a[3] * b[0] * B + a[2] * b[1] * B + a[1] * b[2] * B + a[0] * b[3] * B + uh256(a2);
         requires a14== a[3] * b[1] + a[2] * b[2] + a[1] * b[3] + 
-            a[3] * b[2] * B + a[2] * b[3] * B + uh(a9);
-        requires a15 == a[3] * b[3] + uh(a14);
+            a[3] * b[2] * B + a[2] * b[3] * B + uh256(a9);
+        requires a15 == a[3] * b[3] + uh256(a14);
 
-        requires c_01 == lh(a2);
-        requires c_23 == lh(a9);
-        requires d_01 == lh(a14);
+        requires c_01 == lh256(a2);
+        requires c_23 == lh256(a9);
+        requires d_01 == lh256(a14);
         requires d_23 == a15;
 
         ensures c_01 + c_23 * B2 + d_01 * B4 + d_23 * B6 ==
@@ -112,31 +108,31 @@ module MultiplyExpr256 {
 
         var g2 :int := a[3] as int * b[3];
 
-        assert a9 == g0 + uh(a2);
-        assert a14 == g1 + uh(a9);
-        assert a15 == g2 + uh(a14);
+        assert a9 == g0 + uh256(a2);
+        assert a14 == g1 + uh256(a9);
+        assert a15 == g2 + uh256(a14);
 
         calc == {
             c_01 + c_23 * B2 + d_01 * B4 + d_23 * B6;
-            c_01 + c_23 * B2 + d_01 * B4 + (g2 + uh(a14)) * B6;
-            c_01 + c_23 * B2 + lh(a14) * B4 + (g2 + uh(a14)) * B6;
-            c_01 + c_23 * B2 + lh(a14) * B4 + g2 * B6 + uh(a14) * B6;
+            c_01 + c_23 * B2 + d_01 * B4 + (g2 + uh256(a14)) * B6;
+            c_01 + c_23 * B2 + lh256(a14) * B4 + (g2 + uh256(a14)) * B6;
+            c_01 + c_23 * B2 + lh256(a14) * B4 + g2 * B6 + uh256(a14) * B6;
             {
-        		split_lemma(a14);
+        		split_lemma_256(a14);
             }
             c_01 + c_23 * B2 + a14* B4 + g2 * B6;
-            c_01 + lh(a9) * B2 + a14* B4 + g2 * B6;
-            c_01 + lh(a9) * B2 + (g1 + uh(a9)) * B4 + g2 * B6;
-            c_01 + lh(a9) * B2 + g1 * B4 + uh(a9) * B4 + g2 * B6;
+            c_01 + lh256(a9) * B2 + a14* B4 + g2 * B6;
+            c_01 + lh256(a9) * B2 + (g1 + uh256(a9)) * B4 + g2 * B6;
+            c_01 + lh256(a9) * B2 + g1 * B4 + uh256(a9) * B4 + g2 * B6;
             {
-        		split_lemma(a9);
+        		split_lemma_256(a9);
             }
             c_01 + a9* B2 + g1 * B4 + g2 * B6;
-            lh(a2) + a9* B2 + g1 * B4 + g2 * B6;
-            lh(a2) + (g0 + uh(a2)) * B2 + g1 * B4 + g2 * B6;
-            lh(a2) + g0 * B2 + uh(a2) * B2 + g1 * B4 + g2 * B6;
+            lh256(a2) + a9* B2 + g1 * B4 + g2 * B6;
+            lh256(a2) + (g0 + uh256(a2)) * B2 + g1 * B4 + g2 * B6;
+            lh256(a2) + g0 * B2 + uh256(a2) * B2 + g1 * B4 + g2 * B6;
             {
-        		split_lemma(a2);
+        		split_lemma_256(a2);
             }
             a2 + g0 * B2 + g1 * B4 + g2 * B6;
             {
